SSA/Experimental/Bits/Fast/FiniteStateMachineNew.lean
@@ -1,0 +1,1139 @@
+import Mathlib.Data.Fintype.Card
+import Mathlib.Data.Fintype.Sum
+import Mathlib.Data.Fintype.Sigma
+import Mathlib.Data.Fintype.Pi
+import Mathlib.Data.Fintype.BigOperators
+import Mathlib.Tactic.Zify
+import Mathlib.Tactic.Ring
+
+import SSA.Experimental.Bits.Fast.Defs
+import SSA.Experimental.Bits.Fast.Circuit
+
+open Sum
+
+section FSM
+variable {σ β σ' β' : Type} {γ : β → Type}
+
+def portingSorryImpl {α : Sort _}  : α := sorryAx α
+
+@[implemented_by portingSorryImpl]
+axiom portingSorryAx {α : Sort _}  : α
+
+namespace BitVec
+
+@[simp]
+theorem getLsbD_append_left (x : BitVec v) (y : BitVec w) (i : Nat)
+    (h : ¬(i < w)) :
+    getLsbD (x ++ y) i = x.getLsbD (i - w) := by
+  simp [getLsbD_append, h]
+
+@[simp]
+theorem getLsbD_append_right (x : BitVec v) (y : BitVec w) (i : Nat)
+    (h : i < w) :
+    getLsbD (x ++ y) i = y.getLsbD i := by
+  simp [getLsbD_append, h]
+
+/-- `appendVector` appends a family of `n` bitvectors, each of which might have
+a different width, together into a bitvector whose length is the sum of lengths
+-/
+def appendVector {ws : Fin n → Nat} (xs : (i : Fin n) → BitVec (ws i)) :
+    BitVec (∑ i, ws i) :=
+  match n with
+  | 0   => 0#_
+  | n+1 =>
+    let x := xs 0
+    (x ++ (appendVector (fun i => xs i.succ))).cast <| by
+      simp [Finset.sum]
+
+/-- `appendVector` appends a family of `n` bitvectors, each of which might have
+a different width, together into a bitvector whose length is the sum of lengths
+-/
+def appendVector' {ws : List Nat} (h : ws.length = n)
+    (xs : (i : Fin n) → BitVec ws[i]) :
+    BitVec (Nat.sum ws) :=
+  match n, ws with
+  | 0, []  => 0#_
+  | n+1, _::ws =>
+    let x := xs 0
+    have h : ws.length = n := portingSorryAx
+    (x ++ (appendVector' h (fun i => xs i.succ)))
+
+/-- Construct a bitvector from a function that maps `i : Fin w` to the
+`i`-th least significant bit -/
+def ofFnLsb (f : Fin w → Bool) : BitVec w :=
+  match w with
+  | 0   => 0#0
+  | _+1 => concat (ofFnLsb (f ∘ Fin.succ)) (f 0)
+
+@[simp] lemma getElem_ofFnLsb (f : Fin w → Bool) (i : Fin w) :
+    (ofFnLsb f)[i.val] = f i := by
+  exact portingSorryAx
+
+@[simp] lemma getLsb'_ofFnLsb (f : Fin w → Bool) :
+    (ofFnLsb f).getLsb' = f := by
+  exact portingSorryAx
+
+end BitVec
+
+namespace Fin
+
+def addToSum (i : Fin (x + y)) : Fin x ⊕ Fin y :=
+  if h : i < y then
+    .inr ⟨i, h⟩
+  else
+    .inl (i.subNat y <| by simp_all)
+
+@[simp] abbrev addInl (i : Fin x) : Fin (x + y) := castAdd y i
+@[simp] abbrev addInr (i : Fin y) : Fin (x + y) := natAdd x i
+
+@[deprecated addCases]
+def addElim (f : Fin x → α) (g : Fin y → α) : Fin (x + y) → α :=
+  addCases f g
+
+def sumOfSigma {f : α → Nat} [Fintype α] (i : Σ a, Fin (f a)) : Fin (∑ a, f a) := by
+  exact portingSorryAx
+
+def sumToSigma {f : α → Nat} [Fintype α] (i : Fin (∑ a, f a)) : Σ a, Fin (f a) := by
+  exact portingSorryAx
+
+end Fin
+
+/-- An `n`-ary product of `Bitstream`s. -/
+def BitStreamProd (n : Nat) : Type := Fin n → BitStream
+
+namespace BitStreamProd
+
+/-- Return the `i`-th stream of `x` -/
+def nthStream (x : BitStreamProd n) (i : Fin n) : BitStream := x i
+
+/-- Get the `i`th least significant bit of each constituent stream -/
+def getLsbs (xs : BitStreamProd n) (i : Nat) : BitVec n :=
+  BitVec.ofFnLsb fun j => xs j i
+
+/-- Get the least significant bit of each constituent stream -/
+def heads (xs : BitStreamProd n) : BitVec n :=
+  BitVec.ofFnLsb fun i => (xs i).head
+
+/-- Drop the least significant bit from each constituent stream,
+returning an n-ary product of each streams tail  -/
+def tails (xs : BitStreamProd n) : BitStreamProd n :=
+  fun i => (xs i).tail
+
+def castLE (h : n ≤ m) : BitStreamProd m → BitStreamProd n :=
+  (· ∘ Fin.castLE h)
+
+section Lemmas
+
+@[simp] lemma getElem_heads (xs : BitStreamProd n) (i : Fin n) :
+    xs.heads[i.val] = (xs i).head := by
+  simp [heads]
+
+@[simp] lemma getElem_getLsbs (xs : BitStreamProd n) (i : Nat) (j : Fin n) :
+    (xs.getLsbs i)[j.val] = xs j i := by
+  simp [getLsbs]
+
+end Lemmas
+
+end BitStreamProd
+
+/--
+`CircuitProd vars n` is a collection of `n` Boolean Circuits, each of which can
+refer to at most `vars` variables.
+
+This morally represents a function from `BitVec vars`
+(i.e., an assignment of a single bit per variable),
+to a `BitVec n` (where each circuit computes a single bit of the output).
+See `CircuitProd.eval`.
+-/
+def CircuitProd (vars n : Nat) : Type := Fin n → Circuit (Fin vars)
+
+namespace CircuitProd
+
+
+/-- Evaluate a `CircuitProd vars n` to the function `BitVec vars → BitVec n`
+it represents.
+
+By convention, we use Little Endian order, which is to say, the `i`th circuit
+will compute the `i`-th least significant bit of the output, and the variable
+with index `i` derives it's assignment from the `i`-th least signicant bit of
+the input.
+-/
+def eval {vars n : Nat}
+    (circuit : CircuitProd vars n) (assignment : BitVec vars) :
+    BitVec n :=
+  BitVec.ofFnLsb fun i =>
+    (circuit i).eval assignment.getLsb'
+
+@[simp] lemma getLsbD_eval (c : CircuitProd vars n) (assignment : BitVec vars)
+    (i : Fin n) :
+    (c.eval assignment)[i.val]
+    = (c i).eval assignment.getLsb' := by
+  simp [eval]
+
+/-- The identity circuit family on `n` bits -/
+def id {n : Nat} : CircuitProd n n :=
+  fun i => Circuit.var true i
+
+@[simp] lemma eval_id {n : Nat} : eval id = (@_root_.id (BitVec n)) := by
+  funext xs
+  simp [eval, id]
+  exact portingSorryAx
+
+def map (f : Fin n → Fin m) (cs : CircuitProd n k) : CircuitProd m k :=
+  fun i => (cs i).map f
+
+@[simp] lemma eval_map (f : Fin n → Fin m) (cs : CircuitProd n k) (xs : BitVec m) :
+    eval (cs.map f) xs = eval cs (.ofFnLsb <| (xs[f ·])) := by
+  simp [eval, map]
+
+/-- Re-interpret a family of circuits with `x` variables as a family with
+`x + y` variables -/
+def addInl : CircuitProd x n → CircuitProd (x + y) n :=
+  portingSorryAx
+/-- Re-interpret a family of circuits with `y` variables as a family with
+`x + y` variables -/
+def addInr : CircuitProd y n → CircuitProd (x + y) n :=
+  portingSorryAx
+
+def sigmaMk {f : Fin x → Nat} {i : Fin x} :
+    CircuitProd (f i) n → CircuitProd (∑ j, f j) n :=
+  portingSorryAx
+
+def append {vars n m} (xs : CircuitProd vars n) (ys : CircuitProd vars m) :
+    CircuitProd vars (n + m) := by
+  exact portingSorryAx
+instance : HAppend (CircuitProd vars n) (CircuitProd vars m)
+    (CircuitProd vars (n+m)) where
+  hAppend := append
+
+@[simp] lemma eval_append {vars n m}
+    (xs : CircuitProd vars n) (ys : CircuitProd vars m) (V : BitVec vars) :
+    eval (append xs ys) V = (eval xs V) ++ (eval ys V) := by
+  exact portingSorryAx
+
+#check Circuit.bind
+
+-- def bind (cs : CircuitProd n k) (f : Fin n → CircuitProd )
+
+instance : Subsingleton (CircuitProd n 0) :=
+  inferInstanceAs (Subsingleton (Fin 0 → _))
+
+end CircuitProd
+
+/-- `FSM arity` represents a function `BitStream → ⋯ → BitStream → BitStream`,
+where `arity` is the number of `BitStream` arguments,
+as a finite state machine.
+-/
+structure FSM (arity : Nat) : Type 1 :=
+  /--
+  `stateWidth` is the number of bits the state has
+  -/
+  (stateWidth : Nat)
+  /--
+  `initialState` is the initial state.
+  -/
+  (initialState : BitVec stateWidth)
+  /--
+  `outCircuit` is a single Boolean circuit,
+  which will compute the output bit of the current state,
+  given the current state and input bits.
+  -/
+  (outCircuit : Circuit (Fin <| stateWidth + arity))
+  /--
+  `nextStateCircuit` is a uniform family of `stateWidth` Boolean circuits,
+  where each circuit computes one bit of the next state,
+  given the current state and input bits.
+  -/
+  (nextStateCircuits : CircuitProd (stateWidth + arity) stateWidth)
+
+namespace FSM
+
+/-- A `State` of FSM `p` is just a bitvector with `p.stateWidth` bits -/
+abbrev State (p : FSM arity) : Type := BitVec p.stateWidth
+
+@[deprecated BitVec.append]
+def appendInput {p : FSM arity} (s : BitVec p.stateWidth) (x : BitVec arity) :
+    BitVec (p.stateWidth + arity) :=
+  s ++ x
+
+variable {arity : Nat} (p : FSM arity)
+
+/-- Return the output bit of FSM `p`, given the current state and input bits. -/
+@[simp]
+def outBit (state : p.State) (input : BitVec arity) : Bool :=
+  (p.outCircuit).eval (state ++ input).getLsb'
+
+/-- Return the next state of FSM `p`, given the current state and input bits. -/
+@[simp]
+def nextState (s : p.State) (input : BitVec arity) : p.State :=
+  p.nextStateCircuits.eval (s ++ input)
+
+/-- `p.next state in` computes both the next state bits and the output bit,
+where `state` are the *current* state bits, and `in` are the current input bits. -/
+@[simp]
+def next (state : p.State) (inputBits : BitVec arity) : p.State × Bool :=
+    let newState := p.nextState state inputBits
+    let outBit   := p.outBit state inputBits
+    (newState, outBit)
+
+-- TODO: document this
+def outputStreamAux (s₀ : p.State) (inputStream : BitStreamProd arity) : BitStream := fun n =>
+  match n with
+  | 0 => p.outBit s₀ inputStream.heads
+  | n+1 => outputStreamAux (nextState p s₀ (inputStream.heads)) inputStream.tails n
+
+@[simp]
+theorem outputStreamAux_zero (s₀ : p.State) (inputStream : BitStreamProd arity) :
+    outputStreamAux p s₀ inputStream 0 = p.outBit s₀ (inputStream.getLsbs 0) := rfl
+
+@[simp]
+theorem outputStreamAux_succ (s₀ : p.State) (inputStream : BitStreamProd arity) (n : ℕ) :
+    outputStreamAux p s₀ inputStream (n+1) =
+    outputStreamAux p (p.nextState s₀ (inputStream.heads)) inputStream.tails n := by rfl
+
+/--
+A `StateStream` w.r.t. FSM `p` is an infinite stream of `p.State`s
+-/
+def StateStream (p : FSM arity) := ℕ → p.State
+
+/-- `p.stateStream` is the stream of states of FSM `p`,
+for a given product of input streams.
+
+That is, it is the stream that starts with `p.initialState`,
+and evolves according to `p.nextState`. -/
+def stateStream (p : FSM arity) (xs : BitStreamProd arity) : p.StateStream
+  | 0 => p.initialState
+  | n+1 => (p.nextState (p.stateStream xs n) (xs.getLsbs n))
+
+@[simp]
+theorem stateStream_zero (xs : BitStreamProd arity) :
+    p.stateStream xs 0 = p.initialState := rfl
+
+@[simp]
+theorem stateStream_succ (inputStream : BitStreamProd arity) (n : Nat) :
+    p.stateStream inputStream (n+1)
+    = p.nextState (p.stateStream inputStream n) (inputStream.getLsbs n) :=
+  rfl
+
+-- /-- `eval p` morally gives the function `BitStream → ... → BitStream` represented by FSM `p` -/
+-- def eval (xs : BitStreamProd arity) : BitStream :=
+--   p.outputStreamAux p.initialState xs
+
+def eval.next (xs : BitStreamProd arity × p.State) :
+    (BitStreamProd arity × p.State) × Bool := -- (fun ⟨x, (state : p.State)⟩ =>
+  let x       := xs.1
+  let state   := xs.2
+  let x_head  := x.heads
+  let next    := p.next state x_head
+  let x_tail  := x.tails
+  ((x_tail, next.fst), next.snd)
+
+/-- `eval'` is an alternative definition of `eval`, written in terms of corecursion.  -/
+def eval (x : BitStreamProd arity) : BitStream :=
+  BitStream.corec (eval.next p) (x, p.initialState)
+
+-- /--
+-- Generalized hypothesis that shows how the output stream and
+-- its corecursive definition evolve with an arbitrary input state.
+-- -/
+-- theorem eval_eq_eval'_aux (i : Nat) :
+--     (p.outputStreamAux state x) i = (BitStream.corec (eval'Corec p) (x, state)) i := by
+--   induction i generalizing state x
+--   case zero => rfl
+--   case succ i ih =>
+--     simp [outputStreamAux, eval'Corec, BitStream.corec_succ]
+--     rw [← ih]
+--     rfl
+
+-- /-- Show that the two definitions of evaluation are equivalent. -/
+-- theorem eval_eq_eval' : p.eval x = p.eval' x := by
+--   funext i
+--   apply eval_eq_eval'_aux
+
+/-- `p.withInitialState s` yields an FSM with `s` as the initial state -/
+def withInitialState (p : FSM arity) (s : p.State) : FSM arity :=
+  { p with initialState := s }
+
+theorem eval_withInitialState_succ
+    (p : FSM arity) (c : p.State) (xs : BitStreamProd arity) (n : ℕ) :
+    (p.withInitialState c).eval xs (n+1) =
+      (p.withInitialState (p.nextState c xs.heads)).eval (xs.tails) n := by
+  simp [eval, withInitialState, next]; rfl
+
+
+-- /-- `p.changeVars f` changes the arity of an `FSM`.
+-- The function `f` determines how the new input bits map to the input expected by `p` -/
+-- def changeVars {newArity : Nat} (changeVars : Fin arity → Fin newArity) :
+--     FSM newArity :=
+--   let map (x : BitVec newArity) : BitVec arity :=
+--     BitVec.ofFnLsb (fun j => x[changeVars j])
+--   { p with
+--     outCircuit := p.outCircuit.map _
+--     -- nextBitCirc := fun a => (p.nextBitCirc a).map (Sum.map id changeVars) }
+
+-- open Fin in
+-- def composeUnary (p : FSM 1) (q : FSM n) : FSM n where
+--   stateWidth := p.stateWidth + q.stateWidth
+--   initialState := p.initialState ++ q.initialState
+--   outCircuit := p.outCircuit.bind <| addCases
+--     (fun i => Circuit.var true (addInl <| addInl i))
+--     (fun _ => q.outCircuit.map fun j =>
+--       j.natAdd p.stateWidth |>.cast (by ac_rfl)
+--     )
+--   nextStateCircuits :=
+--    addCases
+--     (fun i => (p.nextStateCircuits i).bind <| )
+--     _
+--     -- p.nextStateCircuits
+
+-- /-- A product of `n` FSMs with the same arity `arity`  -/
+-- def FSMProd (n arity : Nat) : Type 1 :=
+--   Fin n → FSM arity
+
+-- def FSMProd.outCircuits (ps : FSMProd n arity) : CircuitProd _ _ :=
+--   fun i => (ps i).outCircuit
+
+open Fin in
+/--
+Given an FSM `p` of some `arity`,
+and a family of `arity` FSMs `qᵢ`,
+whose (possibly differing) arities are bounded by `newArity`,
+we can compose `p` with `qᵢ` yielding a single FSM of arity `newArity`.
+
+The input of the composed FSM is given to the FSMs `qᵢ`, each of which computes
+a single bit of the input that is then given to `p`. -/
+def compose {newArity : Nat} {qArity : Fin arity → Nat}
+    (vars : ∀ {a : Fin arity}, Fin (qArity a) → Fin newArity)
+    (q : (a : Fin arity) → FSM (qArity a)) :
+    FSM newArity :=
+  let qOutCircuit : CircuitProd
+      ((p.stateWidth + ∑ i : Fin arity, (q i).stateWidth) + newArity)
+      arity :=
+    fun (i : Fin arity) =>
+      (q i).outCircuit.bind <| CircuitProd.append
+        (CircuitProd.id |>.sigmaMk.addInr.addInl)
+        (CircuitProd.id |>.map vars |>.addInr)
+  { stateWidth    := p.stateWidth + (∑ i, (q i).stateWidth),
+    initialState  := p.initialState ++ (BitVec.appendVector (q · |>.initialState))
+    outCircuit :=
+      p.outCircuit.bind <| CircuitProd.append
+        (CircuitProd.id |>.addInl.addInl)
+        qOutCircuit
+    nextStateCircuits :=
+      CircuitProd.append
+        (fun i => (p.nextStateCircuits i).bind <| CircuitProd.append
+          (CircuitProd.id |>.addInl.addInl)
+          qOutCircuit
+        )
+        (fun i =>
+          let ⟨i, j⟩ := i.sumToSigma
+          ((q i).nextStateCircuits j).map <| Fin.addCases
+            (fun k => addInl (addInr (sumOfSigma ⟨_, k⟩)))
+            (fun k => addInr (vars k))
+        )
+  }
+
+/--
+info: 'FSM.compose' depends on axioms: [portingSorryAx, propext, Classical.choice, Quot.sound]
+-/
+#guard_msgs in #print axioms compose
+
+lemma stateStream_compose {newArity : Nat} {qArity : Fin arity → Nat}
+    (vars : ∀ {a : Fin arity}, Fin (qArity a) → Fin newArity)
+    (q : ∀ (i : Fin arity), FSM (qArity i))
+    (xs : BitStreamProd newArity)
+    (n : Nat) :
+    (p.compose vars q).stateStream xs n =
+      let pState := p.stateStream (fun i =>
+        (q i).eval (fun j => xs <| vars j)) n
+      let qState : BitVec (∑ i, (q i).stateWidth) :=
+        BitVec.appendVector fun i =>
+          ((q i).stateStream (fun j => xs <| vars j) n)
+      pState ++ qState := by
+  induction n with
+  | zero => simp [stateStream, compose]
+  | succ n ih =>
+      rw [stateStream, ih]
+      ext (y : Fin (_ + _))
+      cases y using Fin.addCases
+      · simp [stateStream, next, compose, Circuit.eval_bind, eval,
+          CircuitProd.eval, CircuitProd.append]
+        congr
+        ext (z : Fin (_ + _))
+        cases z using Fin.addCases
+        · simp;
+          sorry
+        · simp [Circuit.eval_map, stateStream]
+          congr
+          ext (s : Fin (_ + _))
+          cases s using Fin.addCases
+          · simp; sorry
+          · simp; sorry
+      · simp [Circuit.eval_map, stateStream, compose, eval, next]
+        congr
+        ext (z : Fin (_ + _))
+        cases z using Fin.addCases
+        · simp; sorry
+        · simp; sorry
+
+/-- Evaluating a composed fsm is equivalent to composing the evaluations of the constituent FSMs -/
+lemma eval_compose {newArity : Nat} {qArity : Fin arity → Nat}
+    (arityLE : ∀ (i : Fin arity), qArity i ≤ newArity)
+    (q : ∀ (i : Fin arity), FSM (qArity i))
+    (x : BitStreamProd newArity) :
+    (p.compose arityLE q).eval x =
+      p.eval (λ a => (q a).eval (fun i => x (i.castLE <| arityLE _))) := by
+  ext n
+  stop
+  rw [eval, stateStream_compose, eval]
+  simp [compose, next, Circuit.eval_bind]
+  congr
+  ext a
+  cases a
+  simp
+  simp [Circuit.eval_map, eval, next]
+  congr
+  ext a
+  cases a
+  simp
+  simp
+
+/-!
+## Concrete FSMs
+From here on out, we start to implement various operations as concrete FSMs
+-/
+
+/-! ### Bitwise operations -/
+
+/-- `mapCircuit` lifts a Boolean circuit into a stateless FSM -/
+def mapCircuit (c : Circuit (Fin n)) : FSM n where
+  stateWidth := 0
+  initialState := 0#0
+  outCircuit := c.map (Fin.cast <| by ac_rfl)
+  nextStateCircuits := Fin.elim0
+
+@[simp] lemma eval_mapCircuit (c : Circuit (Fin n)) (xs : BitStreamProd n) :
+    (mapCircuit c).eval xs = (fun n => c.eval fun j => (xs.getLsbs n)[j.val]) := by
+  funext m
+  simp only [eval, mapCircuit]
+  induction m generalizing xs
+  case zero =>
+    simp [eval.next, next, BitVec.zero_width_append _, BitStream.head]
+  case succ m ih =>
+    simp [eval.next]
+    specialize ih xs.tails
+    simp at ih
+    -- rw [ih (xs.tails)]
+
+    sorry
+
+
+
+def and : FSM 2 :=
+  mapCircuit (Circuit.and
+    (Circuit.var true 1)
+    (Circuit.var true 0))
+
+@[simp] lemma eval_and (xs : BitStreamProd 2) :
+    and.eval x = (xs 1) &&& (xs 0) := by
+  ext n;
+  -- stop
+  cases n <;> simp [mapCircuit, and, eval, next]
+
+def or : FSM 2 :=
+  mapCircuit (Circuit.or
+    (Circuit.var true 1)
+    (Circuit.var true 0))
+
+@[simp] lemma eval_or (x : Bool → BitStream) : or.eval x = (x true) ||| (x false) := by
+  ext n; cases n <;> simp [and, eval, next]
+
+def xor : FSM 2 :=
+  mapCircuit (Circuit.xor
+    (Circuit.var true 1)
+    (Circuit.var true 0))
+
+@[simp] lemma eval_xor (xs : BitStreamProd 2) :
+    xor.eval xs = (xs 1) ^^^ (xs 0) := by
+  ext n; stop cases n <;> simp [and, eval, next]
+
+/-! ### Arithmetic -/
+
+def add : FSM 2 where
+  stateWidth := 1
+  initialState := 0#1
+  outCircuit :=
+    Circuit.var true 0
+    ^^^ Circuit.var true 1
+    ^^^ Circuit.var true 2
+  nextStateCircuits _ :=
+    (Circuit.var true 2 &&& Circuit.var true 1)
+    ||| (Circuit.var true 2  &&& Circuit.var true 0)
+    ||| (Circuit.var true 1 &&& Circuit.var true 0)
+
+/-- The internal state of the `add` FSM agrees with
+the carry bit of addition as implemented on bitstreams -/
+theorem carry_add_succ (xs : BitStreamProd 2) (n : ℕ) :
+    add.stateStream xs (n+1)
+    = BitVec.ofBool ((BitStream.addAux (xs 1) (xs 0) n).2) := by
+  ext (a : Fin 1)
+  obtain rfl : a = (0 : Fin 1) := Fin.fin_one_eq_zero a
+  induction n with
+  | zero      =>
+    simp [stateStream, BitStream.addAux, next, add, BitVec.adcb]
+  | succ n ih =>
+    unfold carry
+    simp [next, ih, Circuit.eval, BitStream.addAux, BitVec.adcb]
+
+@[simp] theorem carry_zero (x : BitStreamProd arity) : carry p x 0 = p.initialState := rfl
+@[simp] theorem initialState_add : add.initialState = (fun _ => false) := rfl
+
+@[simp] lemma eval_add (x : Bool → BitStream) : add.eval x = (x true) + (x false) := by
+  ext n
+  simp only [eval]
+  cases n
+  · show Bool.xor _ _ = Bool.xor _ _; simp
+  · rw [carry_add_succ]
+    conv => {rhs; simp only [(· + ·), BitStream.add, Add.add, BitStream.addAux, BitVec.adcb]}
+    simp [next, eval, add]
+/-!
+We don't really need subtraction or negation FSMs,
+given that we can reduce both those operations to just addition and bitwise complement -/
+
+def sub : FSM Bool :=
+  { σ := Unit,
+    initialState := fun _ => false,
+    nextBitCirc := fun a =>
+      match a with
+      | some () =>
+             (Circuit.var false (inr true) &&& Circuit.var true (inr false)) |||
+             ((Circuit.var false (inr true) ^^^ Circuit.var true (inr false)) &&&
+              (Circuit.var true (inl ())))
+      | none => Circuit.var true (inr true) ^^^
+                Circuit.var true (inr false) ^^^
+                Circuit.var true (inl ()) }
+
+theorem carry_sub (x : Bool → BitStream) : ∀ (n : ℕ), sub.carry x (n+1) =
+    fun _ => (BitStream.subAux (x true) (x false) n).2
+  | 0 => by
+    simp [carry, next, Function.funext_iff, BitStream.subAux, sub]
+  | n+1 => by
+    rw [carry, carry_sub _ n]
+    simp [next, eval, sub, BitStream.sub, BitStream.subAux, Bool.xor_not_left']
+
+@[simp]
+theorem eval_sub (x : Bool → BitStream) : sub.eval x = (x true) - (x false) := by
+  simp only [(· - ·), Sub.sub]
+  ext n
+  cases n
+  · simp [eval, sub, next, BitStream.sub, BitStream.subAux, carry]
+  · rw [eval, carry_sub]
+    simp [next, eval, sub, BitStream.sub, BitStream.subAux]
+
+def neg : FSM Unit :=
+  { σ := Unit,
+    i := by infer_instance,
+    initialState := λ _ => true,
+    nextBitCirc := fun a =>
+      match a with
+      | some () => Circuit.var false (inr ()) &&& Circuit.var true (inl ())
+      | none => Circuit.var false (inr ()) ^^^ Circuit.var true (inl ())  }
+
+theorem carry_neg (x : Unit → BitStream) : ∀ (n : ℕ), neg.carry x (n+1) =
+    fun _ => (BitStream.negAux (x ()) n).2
+  | 0 => by
+    simp [carry, next, Function.funext_iff, BitStream.negAux, neg]
+  | n+1 => by
+    rw [carry, carry_neg _ n]
+    simp [next, eval, neg, BitStream.neg, BitStream.negAux, Bool.xor_not_left']
+
+@[simp] lemma eval_neg (x : Unit → BitStream) : neg.eval x = -(x ()) := by
+  show _ = BitStream.neg _
+  ext n
+  cases n
+  · simp [eval, neg, next, BitStream.neg, BitStream.negAux, carry]
+  · rw [eval, carry_neg]
+    simp [next, eval, neg, BitStream.neg, BitStream.negAux]
+
+def not : FSM Unit :=
+  { σ := Empty,
+    initialState := Empty.elim,
+    nextBitCirc := fun _ => Circuit.var false (inr ()) }
+
+@[simp] lemma eval_not (x : Unit → BitStream) : not.eval x = ~~~(x ()) := by
+  ext; simp [eval, not, next]
+
+def zero : FSM (Fin 0) :=
+  { σ := Empty,
+    initialState := Empty.elim,
+    nextBitCirc := fun _ => Circuit.fals }
+
+@[simp] lemma eval_zero (x : Fin 0 → BitStream) : zero.eval x = BitStream.zero := by
+  ext; simp [zero, eval, next]
+
+def one : FSM (Fin 0) :=
+  { σ := Unit,
+    i := by infer_instance,
+    initialState := λ _ => true,
+    nextBitCirc := fun a =>
+      match a with
+      | some () => Circuit.fals
+      | none => Circuit.var true (inl ()) }
+
+@[simp] theorem carry_one (x : Fin 0 → BitStream) (n : ℕ) :
+    one.carry x (n+1) = fun _ => false := by
+  simp [carry, next, one]
+
+@[simp] lemma eval_one (x : Fin 0 → BitStream) : one.eval x = BitStream.one := by
+  ext n
+  cases n
+  · rfl
+  · simp [eval, carry_one, next]
+
+def negOne : FSM (Fin 0) :=
+  { σ := Empty,
+    i := by infer_instance,
+    initialState := Empty.elim,
+    nextBitCirc := fun _ => Circuit.tru }
+
+@[simp] lemma eval_negOne (x : Fin 0 → BitStream) : negOne.eval x = BitStream.negOne := by
+  ext; simp [negOne, eval, next]
+
+def ls (b : Bool) : FSM Unit :=
+  { σ := Unit,
+    initialState := fun _ => b,
+    nextBitCirc := fun x =>
+      match x with
+      | none => Circuit.var true (inl ())
+      | some () => Circuit.var true (inr ()) }
+
+theorem carry_ls (b : Bool) (x : Unit → BitStream) : ∀ (n : ℕ),
+    (ls b).carry x (n+1) = fun _ => x () n
+  | 0 => by
+    simp [carry, next, Function.funext_iff, ls]
+  | n+1 => by
+    rw [carry, carry_ls _ _ n]
+    simp [next, eval, ls]
+
+@[simp] lemma eval_ls (b : Bool) (x : Unit → BitStream) :
+    (ls b).eval x = (x ()).concat b := by
+  ext n
+  cases n
+  · rfl
+  · simp [carry_ls, eval, next, BitStream.concat]
+
+def var (n : ℕ) : FSM (Fin (n+1)) :=
+  { σ := Empty,
+    i := by infer_instance,
+    initialState := Empty.elim,
+    nextBitCirc := λ _ => Circuit.var true (inr (Fin.last _)) }
+
+@[simp] lemma eval_var (n : ℕ) (x : Fin (n+1) → BitStream) : (var n).eval x = x (Fin.last n) := by
+  ext m; cases m <;> simp [var, eval, carry, next]
+
+def incr : FSM Unit :=
+  { σ := Unit,
+    initialState := fun _ => true,
+    nextBitCirc := fun x =>
+      match x with
+      | none => (Circuit.var true (inr ())) ^^^ (Circuit.var true (inl ()))
+      | some _ => (Circuit.var true (inr ())) &&& (Circuit.var true (inl ())) }
+
+theorem carry_incr (x : Unit → BitStream) : ∀ (n : ℕ),
+    incr.carry x (n+1) = fun _ => (BitStream.incrAux (x ()) n).2
+  | 0 => by
+    simp [carry, next, Function.funext_iff, BitStream.incrAux, incr]
+  | n+1 => by
+    rw [carry, carry_incr _ n]
+    simp [next, eval, incr, incr, BitStream.incrAux]
+
+@[simp] lemma eval_incr (x : Unit → BitStream) : incr.eval x = (x ()).incr := by
+  ext n
+  cases n
+  · simp [eval, incr, next, carry, BitStream.incr, BitStream.incrAux]
+  · rw [eval, carry_incr]; rfl
+
+def decr : FSM Unit :=
+  { σ := Unit,
+    i := by infer_instance,
+    initialState := λ _ => true,
+    nextBitCirc := fun x =>
+      match x with
+      | none => (Circuit.var true (inr ())) ^^^ (Circuit.var true (inl ()))
+      | some _ => (Circuit.var false (inr ())) &&& (Circuit.var true (inl ())) }
+
+theorem carry_decr (x : Unit → BitStream) : ∀ (n : ℕ), decr.carry x (n+1) =
+    fun _ => (BitStream.decrAux (x ()) n).2
+  | 0 => by
+    simp [carry, next, Function.funext_iff, BitStream.decrAux, decr]
+  | n+1 => by
+    rw [carry, carry_decr _ n]
+    simp [next, eval, decr, BitStream.decrAux]
+
+@[simp] lemma eval_decr (x : Unit → BitStream) : decr.eval x = BitStream.decr (x ()) := by
+  ext n
+  cases n
+  · simp [eval, decr, next, carry, BitStream.decr, BitStream.decrAux]
+  · rw [eval, carry_decr]; rfl
+
+theorem evalAux_eq_zero_of_set {arity : Type _} (p : FSM arity)
+    (R : Set (p.σ → Bool)) (hR : ∀ x s, (p.next s x).1 ∈ R → s ∈ R)
+    (hi : p.initialState ∉ R) (hr1 : ∀ x s, (p.next s x).2 = true → s ∈ R)
+    (x : BitStreamProd arity) (n : ℕ) : p.eval x n = false ∧ p.carry x n ∉ R := by
+  simp (config := {singlePass := true}) only [← not_imp_not] at hR hr1
+  simp only [Bool.not_eq_true] at hR hr1
+  induction n with
+  | zero =>
+    simp only [eval, carry]
+    exact ⟨hr1 _ _ hi, hi⟩
+  | succ n ih =>
+    simp only [eval, carry] at ih ⊢
+    exact ⟨hr1 _ _ (hR _ _ ih.2), hR _ _ ih.2⟩
+
+theorem eval_eq_zero_of_set {arity : Type _} (p : FSM arity)
+    (R : Set (p.σ → Bool)) (hR : ∀ x s, (p.next s x).1 ∈ R → s ∈ R)
+    (hi : p.initialState ∉ R) (hr1 : ∀ x s, (p.next s x).2 = true → s ∈ R) :
+    p.eval = fun _ _ => false := by
+  ext x n
+  rw [eval]
+  exact (evalAux_eq_zero_of_set p R hR hi hr1 x n).1
+
+def repeatBit : FSM Unit where
+  σ := Unit
+  initialState := fun () => false
+  nextBitCirc := fun _ =>
+    .or (.var true <| .inl ()) (.var true <| .inr ())
+
+@[simp] theorem eval_repeatBit :
+    repeatBit.eval x = BitStream.repeatBit (x ()) := by
+  unfold BitStream.repeatBit
+  rw [eval_eq_eval', eval']
+  apply BitStream.corec_eq_corec
+    (R := fun a b => a.1 () = b.2 ∧ (a.2 ()) = b.1)
+  · simp [repeatBit]
+  · intro ⟨y, a⟩ ⟨b, x⟩ h
+    simp at h
+    simp [h, next, BitStream.head]
+
+end FSM
+
+structure FSMSolution (t : Term) extends FSM (Fin t.arity) :=
+  ( good : t.evalFin = toFSM.eval )
+
+def composeUnary
+    (p : FSM Unit)
+    {t : Term}
+    (q : FSMSolution t) :
+    FSM (Fin t.arity) :=
+  p.compose
+    (Fin t.arity)
+    _
+    (λ _ => id)
+    (λ _ => q.toFSM)
+
+def composeBinary
+    (p : FSM Bool)
+    {t₁ t₂ : Term}
+    (q₁ : FSMSolution t₁)
+    (q₂ : FSMSolution t₂) :
+    FSM (Fin (max t₁.arity t₂.arity)) :=
+  p.compose (Fin (max t₁.arity t₂.arity))
+    (λ b => Fin (cond b t₁.arity t₂.arity))
+    (λ b i => Fin.castLE (by cases b <;> simp) i)
+    (λ b => match b with
+      | true => q₁.toFSM
+      | false => q₂.toFSM)
+
+def composeBinary'
+    (p : FSM Bool)
+    {n m : Nat}
+    (q₁ : FSM (Fin n))
+    (q₂ : FSM (Fin m)) :
+    FSM (Fin (max n m)) :=
+  p.compose (Fin (max n m))
+    (λ b => Fin (cond b n m))
+    (λ b i => Fin.castLE (by cases b <;> simp) i)
+    (λ b => match b with
+      | true => q₁
+      | false => q₂)
+
+@[simp] lemma composeUnary_eval
+    (p : FSM Unit)
+    {t : Term}
+    (q : FSMSolution t)
+    (x : Fin t.BitStreamProd arity) :
+    (composeUnary p q).eval x = p.eval (λ _ => t.evalFin x) := by
+  rw [composeUnary, FSM.eval_compose, q.good]; rfl
+
+@[simp] lemma composeBinary_eval
+    (p : FSM Bool)
+    {t₁ t₂ : Term}
+    (q₁ : FSMSolution t₁)
+    (q₂ : FSMSolution t₂)
+    (x : Fin (max t₁.arity t₂.arity) → BitStream) :
+    (composeBinary p q₁ q₂).eval x = p.eval
+      (λ b => cond b (t₁.evalFin (fun i => x (Fin.castLE (by simp) i)))
+                  (t₂.evalFin (fun i => x (Fin.castLE (by simp) i)))) := by
+  rw [composeBinary, FSM.eval_compose, q₁.good, q₂.good]
+  ext b
+  cases b <;> dsimp <;> congr <;> funext b <;> cases b <;> simp
+
+instance {σ β : Type} [Fintype σ] [Fintype β] (b : Bool) :
+    Fintype (cond b σ β) := by
+  cases b <;> simp <;> infer_instance
+
+open Term
+
+def termEvalEqFSM : ∀ (t : Term), FSMSolution t
+  | var n =>
+    { toFSM := FSM.var n,
+      good := by ext; simp [Term.evalFin] }
+  | zero =>
+    { toFSM := FSM.zero,
+      good := by ext; simp [Term.evalFin] }
+  | one =>
+    { toFSM := FSM.one,
+      good := by ext; simp [Term.evalFin] }
+  | negOne =>
+    { toFSM := FSM.negOne,
+      good := by ext; simp [Term.evalFin] }
+  | Term.and t₁ t₂ =>
+    let q₁ := termEvalEqFSM t₁
+    let q₂ := termEvalEqFSM t₂
+    { toFSM := composeBinary FSM.and q₁ q₂,
+      good := by ext; simp }
+  | Term.or t₁ t₂ =>
+    let q₁ := termEvalEqFSM t₁
+    let q₂ := termEvalEqFSM t₂
+    { toFSM := composeBinary FSM.or q₁ q₂,
+      good := by ext; simp }
+  | Term.xor t₁ t₂ =>
+    let q₁ := termEvalEqFSM t₁
+    let q₂ := termEvalEqFSM t₂
+    { toFSM := composeBinary FSM.xor q₁ q₂,
+      good := by ext; simp }
+  | ls b t =>
+    let q := termEvalEqFSM t
+    { toFSM := by dsimp [arity]; exact composeUnary (FSM.ls b) q,
+      good := by ext; simp }
+  | Term.not t =>
+    let q := termEvalEqFSM t
+    { toFSM := by dsimp [arity]; exact composeUnary FSM.not q,
+      good := by ext; simp }
+  | add t₁ t₂ =>
+    let q₁ := termEvalEqFSM t₁
+    let q₂ := termEvalEqFSM t₂
+    { toFSM := composeBinary FSM.add q₁ q₂,
+      good := by ext; simp }
+  | sub t₁ t₂ =>
+    let q₁ := termEvalEqFSM t₁
+    let q₂ := termEvalEqFSM t₂
+    { toFSM := composeBinary FSM.sub q₁ q₂,
+      good := by ext; simp }
+  | neg t =>
+    let q := termEvalEqFSM t
+    { toFSM := by dsimp [arity]; exact composeUnary FSM.neg q,
+      good := by ext; simp }
+  | incr t =>
+    let q := termEvalEqFSM t
+    { toFSM := by dsimp [arity]; exact composeUnary FSM.incr q,
+      good := by ext; simp }
+  | decr t =>
+    let q := termEvalEqFSM t
+    { toFSM := by dsimp [arity]; exact composeUnary FSM.decr q,
+      good := by ext; simp }
+  | repeatBit t =>
+    let p := termEvalEqFSM t
+    { toFSM := by dsimp [arity]; exact composeUnary FSM.repeatBit p,
+      good := by ext; simp }
+
+/-!
+FSM that implement bitwise-and. Since we use `0` as the good state,
+we keep the invariant that if both inputs are good and our state is `0`, then we produce a `0`.
+If not, we produce an infinite sequence of `1`.
+-/
+def and : FSM Bool :=
+  { σ := Unit,
+    initialState := fun _ => false,
+    nextBitCirc := fun a =>
+      match a with
+      | some () =>
+             -- Only if both are `0` we produce a `0`.
+             (Circuit.var true (inr false)  |||
+             ((Circuit.var false (inr true) |||
+              -- But if we have failed and have value `1`, then we produce a `1` from our state.
+              (Circuit.var true (inl ())))))
+      | none => -- must succeed in both arguments, so we are `0` if both are `0`.
+                Circuit.var true (inr true) |||
+                Circuit.var true (inr false)
+                }
+
+/-!
+FSM that implement bitwise-or. Since we use `0` as the good state,
+we keep the invariant that if either inputs is `0` then our state is `0`.
+If not, we produce a `1`.
+-/
+def or : FSM Bool :=
+  { σ := Unit,
+    initialState := fun _ => false,
+    nextBitCirc := fun a =>
+      match a with
+      | some () =>
+             -- If either succeeds, then the full thing succeeds
+             ((Circuit.var true (inr false)  &&&
+             ((Circuit.var false (inr true)) |||
+             -- On the other hand, if we have failed, then propagate failure.
+              (Circuit.var true (inl ())))))
+      | none => -- can succeed in either argument, so we are `0` if either is `0`.
+                Circuit.var true (inr true) &&&
+                Circuit.var true (inr false)
+                }
+
+/-!
+FSM that implement logical not.
+we keep the invariant that if the input ever fails and becomes a `1`, then we produce a `0`.
+IF not, we produce an infinite sequence of `1`.
+
+EDIT: Aha, this doesn't work!
+We need NFA to DFA here (as the presburger book does),
+where we must produce an infinite sequence of`0` iff the input can *ever* become a `1`.
+But here, since we phrase things directly in terms of producing sequences, it's a bit less clear
+what we should do :)
+
+- Alternatively, we need to be able to decide `eventually always zero`.
+- Alternatively, we push negations inside, and decide `⬝ ≠ ⬝` and `⬝ ≰ ⬝`.
+-/
+
+inductive Result : Type
+  | falseAfter (n : ℕ) : Result
+  | trueFor (n : ℕ) : Result
+  | trueForall : Result
+deriving Repr, DecidableEq
+
+def card_compl [Fintype σ] [DecidableEq σ] (c : Circuit σ) : ℕ :=
+  Finset.card $ (@Finset.univ (σ → Bool) _).filter (fun a => c.eval a = false)
+
+theorem decideIfZeroAux_wf {σ : Type _} [Fintype σ] [DecidableEq σ]
+    {c c' : Circuit σ} (h : ¬c' ≤ c) : card_compl (c' ||| c) < card_compl c := by
+  apply Finset.card_lt_card
+  simp [Finset.ssubset_iff, Finset.subset_iff]
+  simp only [Circuit.le_def, not_forall, Bool.not_eq_true] at h
+  rcases h with ⟨x, hx, h⟩
+  use x
+  simp [hx, h]
+
+def decideIfZerosAux {arity : Type _} [DecidableEq arity]
+    (p : FSM arity) (c : Circuit p.σ) : Bool :=
+  if c.eval p.initialState
+  then false
+  else
+    have c' := (c.bind (p.nextBitCirc ∘ some)).fst
+    if h : c' ≤ c then true
+    else
+      have _wf : card_compl (c' ||| c) < card_compl c :=
+        decideIfZeroAux_wf h
+      decideIfZerosAux p (c' ||| c)
+  termination_by card_compl c
+
+def decideIfZeros {arity : Type _} [DecidableEq arity]
+    (p : FSM arity) : Bool :=
+  decideIfZerosAux p (p.nextBitCirc none).fst
+
+theorem decideIfZerosAux_correct {arity : Type _} [DecidableEq arity]
+    (p : FSM arity) (c : Circuit p.σ)
+    (hc : ∀ s, c.eval s = true →
+      ∃ m y, (p.withInitialState s).eval y m = true)
+    (hc₂ : ∀ (x : arity → Bool) (s : p.σ → Bool),
+      (FSM.next p s x).snd = true → Circuit.eval c s = true) :
+    decideIfZerosAux p c = true ↔ ∀ n x, p.eval x n = false := by
+  rw [decideIfZerosAux]
+  split_ifs with h
+  · simp
+    exact hc p.initialState h
+  · dsimp
+    split_ifs with h'
+    · simp only [true_iff]
+      intro n x
+      rw [p.eval_eq_zero_of_set {x | c.eval x = true}]
+      · intro y s
+        simp [Circuit.le_def, Circuit.eval_fst, Circuit.eval_bind] at h'
+        simp [Circuit.eval_fst, FSM.next]
+        apply h'
+      · assumption
+      · exact hc₂
+    · let c' := (c.bind (p.nextBitCirc ∘ some)).fst
+      have _wf : card_compl (c' ||| c) < card_compl c :=
+        decideIfZeroAux_wf h'
+      apply decideIfZerosAux_correct p (c' ||| c)
+      simp [c', Circuit.eval_fst, Circuit.eval_bind]
+      intro s hs
+      rcases hs with ⟨x, hx⟩ | h
+      · rcases hc _ hx with ⟨m, y, hmy⟩
+        use (m+1)
+        use fun a i => Nat.casesOn i x (fun i a => y a i) a
+        rw [FSM.eval_withInitialState_succ]
+        rw [← hmy]
+        simp only [FSM.next, Nat.rec_zero, Nat.rec_add_one]
+      · exact hc _ h
+      · intro x s h
+        have := hc₂ _ _ h
+        simp only [Circuit.eval_bind, Bool.or_eq_true, Circuit.eval_fst,
+          Circuit.eval_or, this, or_true]
+termination_by card_compl c
+
+theorem decideIfZeros_correct {arity : Type _} [DecidableEq arity]
+    (p : FSM arity) : decideIfZeros p = true ↔ ∀ n x, p.eval x n = false := by
+  apply decideIfZerosAux_correct
+  · simp only [Circuit.eval_fst, forall_exists_index]
+    intro s x h
+    use 0
+    use (fun a _ => x a)
+    simpa [FSM.eval, FSM.withInitialState, FSM.next, FSM.carry]
+  · simp only [Circuit.eval_fst]
+    intro x s h
+    use x
+    exact h
+
+end FSM
+
+/--
+The fragment of predicate logic that we support in `bv_automata`.
+Currently, we support equality, conjunction, disjunction, and negation.
+This can be expanded to also support arithmetic constraints such as unsigned-less-than.
+-/
+inductive Predicate : Nat → Type _ where
+| eq (t1 t2 : Term) : Predicate ((max t1.arity t2.arity))
+| and  (p : Predicate n) (q : Predicate m) : Predicate (max n m)
+| or  (p : Predicate n) (q : Predicate m) : Predicate (max n m)
+-- For now, we can't prove `not`, because it needs NFA → DFA conversion
+-- the way Sid knows how to build it, or negation normal form,
+-- both of which is machinery we lack.
+-- | not (p : Predicate n) : Predicate n
+
+
+
+/--
+denote a reflected `predicate` into a `prop.
+-/
+def Predicate.denote : Predicate σ → Prop
+| eq t1 t2 => t1.eval = t2.eval
+| and p q => p.denote ∧  q.denote
+| or p q => p.denote ∨  q.denote
+-- | not p => ¬ p.denote
+
+/--
+Convert a predicate into a proposition
+-/
+def Predicate.toFSM : Predicate k → FSM (Fin k)
+| .eq t1 t2 => (termEvalEqFSM (Term.repeatBit <| Term.xor t1 t2)).toFSM
+| .and p q =>
+    let p := toFSM p
+    let q := toFSM q
+    composeBinary' FSM.and p q
+| .or p q =>
+    let p := toFSM p
+    let q := toFSM q
+    composeBinary' FSM.or p q
+
+theorem Predicate.toFsm_correct {k : Nat} (p : Predicate k) :
+  decideIfZeros p.toFSM = true ↔ p.denote := by sorry
